
# Table of Contents

1.  [Lecture #2](#org74563c5)
    1.  [Integration by substitution (Backwards chain rule)](#org063116d)

date: 22-2-24


<a id="org74563c5"></a>

# Lecture #2


<a id="org063116d"></a>

## Integration by substitution (Backwards chain rule)

Solve integration by substituting a part of the function with the condition that the derivative of the part substituted is present and multiplied by $dx$.

-   Examples:
    
    1.  
    
    $$\int \cos(x^2) \times 2x .dx \qquad x^2 = u \rightarrow du = 2x dx$$
    $$\rightarrow \int \cos(u) \times du = \sin(u) + c \rightarrow \sin(x^2) + c$$
    
    2.  
    
    $$\int \frac{1}{x\ln(x)} .dx \qquad ln(x) = u \rightarrow du = \frac{1}{x} dx$$
    
    $$\rightarrow \int \frac{1}{u} .dx = \ln(u) + c \rightarrow \ln(ln(x)) + c$$
    
    3.  
    
    $$\int x^3 \times \sqrt{x^2 + 1} .dx \qquad u = x^2 + 1 \rightarrow du = 2x dx \rightarrow x^2 = u + 1$$
    
    $$\frac{1}{2} \int (u + 1) \times \sqrt{u} du = \frac{1}{2} \int u^{\frac{3}{2}} + u^{\frac{1}{2}} du$$
    
    $$= \frac{1}{2} \times (\frac{u^{\frac{5}{2}}}{\frac{5}{2}} + \frac{u^{\frac{3}{2}}}{\frac{3}{2}}) + c$$

    - then substitute with the original values

