
# Table of Contents

1.  [Assignment #1](#org6391d48)
    1.  [Attempt #1](#orga820ce9)
        1.  [Question 1](#org238655c)
        2.  [Question 2](#org38f1645)
        3.  [Question 3](#org95dd16e)
        4.  [Question 4](#org1dec6da)
        5.  [Question 5](#orge083195)
        6.  [Question 6](#org127bc90)
        7.  [Question 7](#org2ea47f8)
        8.  [Question 8](#orgce796ad)
        9.  [Question 9](#org43e90a4)
        10. [Question 10](#org74b2c76)
        11. [Question 11](#orgc031735)
        12. [Question 17](#orga304d81)
    2.  [Attempt #2](#org4ff84bf)
        1.  [Question 2](#org7793aa1)
        2.  [Question 3](#org64a9eb5)
        3.  [Question 5](#org10f4845)
        4.  [Question 6](#org6e6066a)
        5.  [Question 11](#org4bc7eeb)
        6.  [Question 12](#orgaea1bbf)
        7.  [Question 14](#org035c03c)


<a id="org6391d48"></a>

# Assignment #1


<a id="orga820ce9"></a>

## Attempt #1


<a id="org238655c"></a>

### Question 1

$$\int \frac{1}{1 + e^{2x}} = \tan^{-1}(e^{x}) + c$$

sol:

$$\frac{d}{d_{x}}(\tan^{-1}(e^{x}) + c) = \frac{e^{x}}{e^{2x} + 1}$$

$\therefore$ the relation is true.


<a id="org38f1645"></a>

### Question 2

$$\int \sqrt{\frac{\cosh(x) - \sinh(x)}{\cosh(x) + \sinh(x)}} .dx$$

sol:

$$\int \sqrt{\frac{e^{-x}}{e^{x}}} = \int \sqrt{\frac{1}{e^{2x}}} .dx = \int e^{-x} = -e^{-x} + c$$


<a id="org95dd16e"></a>

### Question 3

$$\int \frac{1}{\sqrt{2 - x^{2}}} .dx$$

sol:

$$a = \sqrt{2} \rightarrow \arcsin(\frac{x}{\sqrt{2}}) + c$$


<a id="org1dec6da"></a>

### Question 4

$$\int \sqrt{e^{x}} .dx = 2 \sqrt{e^{x}} + c$$

sol:

$$\frac{d}{d_{x}}(2\sqrt{e^{x}} + c) = 2 \times \frac{e^{x}}{2\sqrt{e^{x}}} = \frac{e^{x}}{\sqrt{e^{x}}}$$

$\therefore$ the relation is false.


<a id="orge083195"></a>

### Question 5

$$\int \frac{1}{x \sqrt{x^{2} - 2}} $$

sol:

$$ \frac{1}{\sqrt{2}} \sec^{-1}(\frac{x}{\sqrt{2}}) + c $$


<a id="org127bc90"></a>

### Question 6

$$\int x \cos(x) .dx = \frac{x^{2}}{2} \times \frac{\cos^{2}(x)}{2} + c$$

sol:

$$ \frac{d}{d_{x}}(\frac{1}{4}\ x^{2} \times \cos^{2}(x) + c) = \frac{1}{4}(x^{2} \times 2\cos(x) \times \sin(x) + \cos^{2}(x) \times 2x) $$

$$ = \frac{1}{4}(x^{2} \times \sin(2x) + \cos^{2}(x) \times 2x) $$


<a id="org2ea47f8"></a>

### Question 7

$$\int \frac{1}{x^{2} + 6x + 13}\ .dx$$

sol:

$$ \int \frac{1}{(x + 3)^{2} + 1} $$


<a id="orgce796ad"></a>

### Question 8

$$ \int (e^{x} + 3^{x})^{2} .dx$$

sol:

$$ \int e^{2x} + 3^{2x} + 2 \times e^{x} \times 3^{x} .dx $$

$$ = \frac{e^{2x}}{2} + \frac{3^{2x}}{2\ln(3)} +  $$


<a id="org43e90a4"></a>

### Question 9

$$ \int \frac{1}{\sqrt{x^{2} + 4x + 5}}\ .dx $$

sol:

$$ \int \frac{1}{\sqrt{(x + 2)^{2} + 1}}  $$


<a id="org74b2c76"></a>

### Question 10

$$ \int \frac{1}{4 + 16x^{2}} .dx $$

sol:

$$ \int \frac{1}{16(\frac{1}{4} + x^{2})} .dx = \frac{1}{16} \times 2 \arctan(\frac{2x}{1}) + c $$


<a id="orgc031735"></a>

### Question 11

$$ \int \frac{\cosh(x)}{\sqrt{\sinh^{2}(x) - 2\sinh(x)}} .dx$$

sol:


<a id="orga304d81"></a>

### Question 17

$$\int \sinh(\ln(x)) .dx$$

sol:


<a id="org4ff84bf"></a>

## Attempt #2


<a id="org7793aa1"></a>

### Question 2

$$\int \frac{1}{\sqrt{x^{2}+2x}$$

sol:

$$\int \frac{1}{\sqrt{(x + 1)^{2} - 1}}$$


<a id="org64a9eb5"></a>

### Question 3

$$ \int \frac{1}{\sqrt{2x^{2} + 1}} $$

sol:

$$ \frac{1}{\sqrt{2}} \int \frac{1}{\sqrt{x^{2} + \frac{1}{2}}} $$


<a id="org10f4845"></a>

### Question 5

$$\int \frac{e^{x}}{\sqrt{e^{2x}-2e^{x}}}$$

sol:

$$\int \frac{e^{x}}{e^{x} \times \sqrt{1-2e^{-x}}} = \int \frac{1}{\sqrt{1-2e^{-x}}} $$


<a id="org6e6066a"></a>

### Question 6

$$ \int (\cos(x) + \sin(x))^2 $$

sol:

$$ \int 1 + \sin(2x) $$


<a id="org4bc7eeb"></a>

### Question 11

$$ \int \frac{1}{\sinh^{2}(7x)} $$

sol:

$$ \int \csch^{2}(7x) = -\frac{\coth(7x)}{7} + c$$


<a id="orgaea1bbf"></a>

### Question 12

$$ \int \frac{1}{4-16x^{2}} $$

sol:

$$ \frac{1}{16} \int \frac{1}{(\frac{1}{4}-x^{2})} = \frac{1}{16} \times 2 \tanh^{-1}(2x) $$


<a id="org035c03c"></a>

### Question 14

$$ \int \frac{1}{(\cosh(x) + \sinh(x))^{2}} $$

sol:

$$ \int \frac{1}{e^{2x}} = \int e^{-2x} = -\frac{1}{2} e^{-2x} $$

